Added a recursive definition for executing a small step.
It returns TPHang if no small step can be executed.  This is currently
not consistent with the inductive definition, which does not implement
any handling of hanging excutions.

The best way to fix this might be create a definition that clearly
states, that a small step is only possible, if the result of applying
smallstep to the expression is *not* TPHang.  Using this definition, it
should be possible to show, that the inductive definition is consistent
with the recursive definition of small steps.

TPSmallSteps.v
@@ -35,20 +35,9 @@ Fixpoint TPFreeVars exp :=
     | TPExpRec id exp => filter (ident_eq id) (TPFreeVars exp)
   end.
 
-(*
-Fixpoint subst free_ids e e' id :=
-  match e with
-    | TPConstant c => c
-    | TPExpId id' => if string_eq id' id then e' else id'
-    | TPExpAbstr id' e => if string_eq id' id then e else
-      let id'' := new_id free_ids id' in TPExpAbstr id'' (subst (id'' :: free_ids) (subst free_ids e' (TPExpId id'') id) e' id)
-    | _ => TPConstant TPunit
-  end.
-*)
-
 Definition new_id highest_id id := (TPId (id, S highest_id), S highest_id).
 
-(* Substitute id in e by e' *)
+(* Substitute id in e by e', using notation from lecture: e[e'/id] *)
 Fixpoint TPSubst (highest_id : nat) e e' id : TPExp * nat :=
   match e with
     | TPExpConst c => (e, highest_id)
@@ -98,7 +87,37 @@ Inductive TPMakesSmallstep: nat -> TPExp -> TPExp * nat -> Prop :=
 | smallstep_leteval: forall idx idx' id exp1 exp1' exp2,
   TPMakesSmallstep idx exp1 (exp1', idx') -> TPMakesSmallstep idx' (TPLet id exp1 exp2) (TPLet id exp1' exp2, idx')
 | smallstep_letexec: forall idx id exp v,
-  TPIsValue v -> TPMakesSmallstep idx (TPLet id v exp) (TPSubst idx exp v id).
+  TPIsValue v -> TPMakesSmallstep idx (TPLet id v exp) (TPSubst idx exp v id)
+| smallstep_unfold: forall idx id exp,
+  TPMakesSmallstep idx (TPRec id exp) (TPSubst idx exp (TPRec id exp) id).
+
+Fixpoint smallstep (n : nat) (exp : TPExp) : TPExp * nat :=
+  match exp with
+    | TPExpApp (TPExpApp (TPExpConst (TPConstantOp op)) (TPExpConst (TPConstantInt n1))) (TPExpConst (TPConstantInt n2)) =>
+      (TPEvalOp op (TPInt n1) (TPInt n2), n)                                  (* OP *)
+    | TPExpApp (TPExpAbstr id e1) e2 =>
+      if TPIsValue_bool e2
+        then TPSubst n e1 e2 id                                               (* BETA-V *)
+        else let (e', n') := smallstep n e2 in (TPApp (TPAbstr id e1) e', n') (* APP-RIGHT *)
+    | TPExpApp e1 e2 =>
+      if TPIsValue_bool e1
+        then let (e', n') := smallstep n e2 in (TPApp e1 e', n')              (* APP-LEFT *)
+        else let (e', n') := smallstep n e1 in (TPApp e' e2, n')              (* APP-RIGHT *)
+    | TPExpIf e1 e2 e3 =>
+      if TPIsValue_bool e1
+        then if TPExp_eq e1 TPTrue
+          then (e2, n)                                                        (* COND-TRUE *)
+          else (e3, n)                                                        (* COND-FALSE *)
+        else let (e', n') := smallstep n e1 in (TPIf e' e2 e3, n')            (* COND-EVAL *)
+    | TPExpLet id e1 e2 =>
+      if TPIsValue_bool e1
+        then TPSubst n e2 e1 id                                               (* LET-EXEC *)
+        else let (e', n') := smallstep n e1 in (TPLet id e' e2, n')           (* LET-EVAL *)
+    | TPExpRec id e => TPSubst n e (TPRec id e) id                            (* UNFOLD *)
+  (* Otherwise, no small step exists and the execution hangs *)
+    | _ => (TPHang, n)
+  end.
+
 
 Inductive NonEmptyList (A: Type) :=
 | Singleton: A -> NonEmptyList A
@@ -185,6 +204,14 @@ Proof.
   now apply TPAbstrIsValue.
   apply smallstep_op.
 Qed.
+
+Lemma smallstep_consist : forall n n' e e', smallstep n e = (e', n') <-> TPMakesSmallstep n e (e', n').
+Proof.
+  intros n n' e e'.
+  induction e.
+  unfold smallstep.
+Admitted.
+
 
 End TPSmallSteps.
 
